Introduced tvalue: type

src/ast/env_graph_gc.v
@@ -5,6 +5,8 @@ From CertiGC Require Export ast.clightgen.gc.
 Instance CompSpecs : compspecs. make_compspecs prog. Defined.
 Definition Vprog : varspecs. mk_varspecs prog. Defined.
 
+Definition tvalue: type := tptr tvoid.
+
 Definition thread_info_type : type := Tstruct _thread_info noattr.
 Definition space_type : type := Tstruct _space noattr.
 Definition heap_type: type := Tstruct _heap noattr.
