src/proof/verif_conversion.v
@@ -5,7 +5,11 @@ Lemma body_int_to_int_or_ptr:
 Proof.
   start_function.
   forward.
-Qed.
+  destruct x ; try easy.
+  unfold denote_tc_iszero, valid_int_or_ptr in *. cbv [Archi.ptr64] in *.
+  unfold is_true.
+  admit.
+Admitted.
 
 Lemma body_int_or_ptr_to_int:
   semax_body Vprog Gprog f_int_or_ptr_to_int int_or_ptr_to_int_spec.
