src/proof/verif_forward_roots.v
@@ -61,27 +61,25 @@ Proof.
       remember (Znth i (live_roots_indices f_info)).
       replace_SEP 1 (fun_info_rep rsh f_info fi) by entailer.
       assert_PROP (force_val
-                     (if Archi.ptr64 then
-                        (sem_add_ptr_long
-                           int_or_ptr_type (offset_val 24 ti) (Z2val z)) else
-                        (sem_add_ptr_int int_or_ptr_type
-                                         Unsigned (offset_val 12 ti) (Z2val z))) =
-                   field_address thread_info_type
-                                 [ArraySubsc z; StructField _args] ti). {
+                     (if Archi.ptr64
+                        then (sem_add_ptr_long tvalue (offset_val 24 ti) (Z2val z))
+                        else (sem_add_ptr_int tvalue Unsigned (offset_val 12 ti) (Z2val z)))
+                      = field_address thread_info_type [ArraySubsc z; StructField _args] ti
+      ).
+      {
         unfold thread_info_rep. Intros. entailer!. simpl. unfold Z2val.
         first [rewrite sem_add_pi_ptr_special' |
                rewrite sem_add_pl_ptr_special] ; auto. simpl. unfold field_address.
         rewrite if_true. 1: simpl; rewrite offset_offset_val; reflexivity.
-        unfold field_compatible in *. simpl. unfold in_members. simpl. intuition. }
-      assert (Zlength roots' = Zlength roots) by
-          (apply frl_roots_Zlength in H8; assumption).
-      forward_call (rsh, sh, gv, fi, ti, g', t_info', f_info, roots', outlier, from,
-                    to, 0, (@inl _ (Addr*Z) i)).
+        unfold field_compatible in *. simpl. unfold in_members. simpl. intuition.
+      }
+      assert (Zlength roots' = Zlength roots) by (apply frl_roots_Zlength in H8; assumption).
+      forward_call (rsh, sh, gv, fi, ti, g', t_info', f_info, roots', outlier, from, to, 0, (@inl _ (Addr*Z) i)).
       * simpl snd. apply prop_right.
-        change (Tpointer tvoid {| attr_volatile := false; attr_alignas := Some 2%N |})
-          with int_or_ptr_type.
-        change (Tpointer tvoid {| attr_volatile := false; attr_alignas := Some 3%N |})
-          with int_or_ptr_type. simpl. cbv [Archi.ptr64] in H14. rewrite H14.
+        change (Tpointer tvoid {| attr_volatile := false; attr_alignas := Some 2%N |}) with tvalue.
+        change (Tpointer tvoid {| attr_volatile := false; attr_alignas := Some 3%N |}) with tvalue.
+        change (tptr tvoid) with tvalue.
+        simpl. cbv [Archi.ptr64] in H14. rewrite H14.
         rewrite <- Heqz. clear. intuition.
       * intuition. red. rewrite H15, H5. split; assumption.
       * Intros vret. destruct vret as [[g2 t_info2] roots2]. simpl fst in *.
